\documentclass[a4paper]{article}

%Russian-specific packages
%--------------------------------------
\usepackage[T2A]{fontenc}
\usepackage[utf8]{inputenc}
\usepackage[english, russian]{babel}
%for search in russian
\usepackage{cmap}
%--------------------------------------

%Math-specific packages
%--------------------------------------
\usepackage{amsmath}
\usepackage{amssymb}
\usepackage{hyperref}

%Format-specific packages
%--------------------------------------
\usepackage[left=1cm,
            right=1cm,
            top=1cm,
            bottom=1cm,
            bindingoffset=0cm]{geometry}
%--------------------------------------

% for theorems, lemmas and definitions
%--------------------------------------
\usepackage{amsthm}

\newtheorem{theorem}{Теорема}

\theoremstyle{definition}
\newtheorem {definition}{Опрeделение}
\newtheorem {task}{Задача}

%--------------------------------------

%Roman enum items
\usepackage{enumerate}

% For graphics
%--------------------------------------
\usepackage{tikz}
\usetikzlibrary{
  % for faster compilation
  external
  % for cool arrows
  , arrows.meta
  % for angles
  , angles
  , quotes
  , babel
}
\tikzsetexternalprefix{tasks/}
\tikzexternalize

%--------------------------------------

% My commands
%--------------------------------------

\DeclareMathOperator{\sgn}{sgn}

\def\const{ \mathrm{const} }
\def\eps{ \varepsilon }
\def\Eps{ \mathcal{E} }

\def\R{ \mathbb{R} }
\def\Z{ \mathbb{Z} }
\def\C{ \mathbb{C} }
\def\E{ \mathrm{E} }
\def\D{ \mathrm{D} }
\def\P{ \mathrm{P} }

\def\littleO{ \overline{\overline{o}} }
\def\bigO{ \underline{\underline{\mathcal{O}}} }

\newcommand*{\norm}[1]{\left\lVert#1\right\rVert}
\newcommand*{\abs}[1]{\left\lvert#1\right\rvert}

\date{Осенний семестр 2023}
\title{Некоторые доказательства}

% suppress page count
\pagestyle{empty}



\begin{document}


\begin{theorem}
    In the regression:                                                                                                                                                                                                                                                                                                                                                                                        
    \begin{equation*}
        \frac{\Delta A_{k+2}}{\Delta t_{k+2}} - \frac{\Delta A_{k+1}}{\Delta t_{k+1}} 
    = - \rho \Delta A_{k+1} + \rho \lambda x_{t_{k+1}} + 
    (\kappa + \lambda) (\frac{x_{t_{k+2}}}{\Delta t_{k+2}} - \frac{x_{t_{k+1}}}{\Delta t_{k+1}}).
    \end{equation*}
    the coefficients $\rho, \kappa$ and $\lambda$ the same as in OW model describes the market with dynamics
    describing by series $A_k, \Delta t _k, x_k$.

Here:
\begin{itemize}
\item $x_{k}$ 
--- the trade size at $t_k$.
\item $A_{k}$ --- ask price at $t_k$. 
\end{itemize}

\end{theorem}
\begin{proof}
From the definitions of the model follows three equations:
\begin{equation} \label{rp1}
    A_{t_k} = V_{t_k} + \frac{s}{2} + \sum _{i=0} ^{k-1} x_{t_i} \kappa e^{- \rho (t_k - t_i)}
\end{equation}
\begin{equation}\label{rp2}
    V_{t_{k+1}} = V_{t_k} + \lambda x_{t_k} \rightarrow V_{t_{k+1}} - V_{t_k} = \lambda x_{t_{k}}
\end{equation}
\begin{equation} \label{rp3}
    D_{t_k} = A_{t_k} - V_{t_k} - \frac{s}{2}
\end{equation}

From \eqref{rp1} and \eqref{rp3}:
\begin{align*}
    D_{t_k} &= \sum _{i=0} ^{k-1} x_{t_i} \kappa e^{- \rho (t_k - t_i)} \\
    \Delta D_{t_k} &= \sum _{i=0} ^k x_{t_i} \kappa e^{- \rho (t_{k+1} - t_i)} 
    - \sum _{i=0} ^{k - 1} x_{t_i} \kappa e^{- \rho (t_k - t_i)}
    = \sum _{i=0} ^{k - 1} x_{t_i} \kappa (e^{- \rho (t_{k+1} - t_i)} - e^{- \rho (t_k - t_i)})
    + x_{t_i} \kappa e^{- \rho (t_{k+1} - t_k)} = \\
    &= \sum _{i=0} ^{k - 1} x_{t_i} \kappa e^{- \rho (t_k - t_i)} (e^{- \rho (t_{k+1} - t_k)} - 1)
    + x_{t_i} \kappa e^{- \rho (t_{k+1} - t_k)} = 
    [\textrm{considering $e^{- \rho (t_{k +1} - t_k)} = 1 - \rho (t_{k+1} - t_k)$}] = \\
    &=\sum _{i=0} ^{k - 1} x_{t_i} \kappa e^{- \rho (t_k - t_i)} ((1 - \rho (t_{k+1} - t_k)) - 1)
    + x_{t_i} \kappa (1 - \rho (t_{k+1} - t_k)) 
    = - \rho \Delta t_{k} D_{t_k} + x_{t_i} \kappa (1 - \rho \Delta t_{k}).
\end{align*}

On the other hand, from \eqref{rp2} and \eqref{rp3} one has:

\begin{equation*}
    \Delta D_k = D_{k+1} - D_k = A_{k+1} + V_{k+1} - A_{k} - V_{k} = \Delta A_k - \Delta V_k \rightarrow \Delta A_k = \Delta D_k + \Delta V_k .
\end{equation*}

Thus, one has an equation:
\begin{equation*}
    \Delta A_k = - \rho \Delta t_{k} D_{t_k} + x_{t_i} \kappa (1 - \rho \Delta t_{k}) + \lambda x_{t_k} .
\end{equation*} 

But one does not want to deal with $D_{t_k}$, so he divides regression for $\Delta t_k$ and considers 
a divided difference of $A_{t_{k+1}}$ and $A_{t_{k}}$:

\begin{align*}
    \frac{\Delta A_{k+1}}{\Delta t_{k+1}} - \frac{\Delta A_{k}}{\Delta t_{k}} 
    &=- \rho D_{t_{k+1}} + x_{t_{k+1}} \kappa \left(\frac{1}{\Delta t_{k+1}} - \rho \right) + \lambda \frac{x_{t_{k+1}}}{\Delta t_{k+1}}
     + \rho D_{t_{k}}   - x_{t_{k}}   \kappa \left(\frac{1}{\Delta t_{k}} - \rho \right)   - \lambda \frac{x_{t_k}}    {\Delta t_{k}} = \\
    &= -\rho (\Delta A_k - \Delta V_k) + (\lambda + \kappa) \left(\frac{x_{t_{k+1}}}{\Delta t_{k+1}} - \frac{x_{t_k}}{\Delta t_{k}}\right) - \rho \kappa (x_{t_{k+1}} - x_{t_{k}})= \\
    &= -\rho \Delta A_k + \rho (\lambda + \kappa) x_{t_k} - \rho \kappa x_{t_{k+1}} + (\lambda + \kappa) \left(\frac{x_{t_{k+1}}}{\Delta t_{k+1}} - \frac{x_{t_k}}{\Delta t_{k}}\right).
\end{align*} 

\end{proof}

\end{document}